add DFA cache that gets updated dynamically

Parser.v
@@ -443,10 +443,13 @@ Module ParserFn (Import D : Defs.T).
 
   (* cache-optimized version *)
 
+  Definition cache := PC.PEF.P.SLL.cache.
+  Definition empty_cache := PC.PEF.P.SLL.empty_cache.
+
   Inductive step_result_opt :=
   | StepAccept_opt : forest -> step_result_opt
   | StepReject_opt : string -> step_result_opt
-  | StepK_opt      : prefix_stack -> suffix_stack -> list token -> NtSet.t -> bool -> step_result_opt
+  | StepK_opt      : prefix_stack -> suffix_stack -> list token -> NtSet.t -> bool -> cache -> step_result_opt
   | StepError_opt  : parse_error -> step_result_opt.
 
   Definition step_opt (g      : grammar)
@@ -455,7 +458,8 @@ Module ParserFn (Import D : Defs.T).
                       (s_stk  : suffix_stack)
                       (ts     : list token)
                       (av     : NtSet.t)
-                      (u      : bool) : step_result_opt := 
+                      (u      : bool) 
+                      (c      : cache) : step_result_opt := 
     match p_stk, s_stk with
     | (PF pre v, p_frs), (SF suf, s_frs) =>
       match suf with
@@ -476,7 +480,8 @@ Module ParserFn (Import D : Defs.T).
           | NT x :: suf_cr'   =>
             let p_stk' := (PF (NT x :: pre_cr) (Node x (rev v) :: v_cr), p_frs') in
             let s_stk' := (SF suf_cr', s_frs')                                   in
-            StepK_opt p_stk' s_stk' ts (NtSet.add x av) u          end
+            StepK_opt p_stk' s_stk' ts (NtSet.add x av) u c          
+          end
         | _, _ => StepError_opt InvalidState
         end
       (* terminal case --> consume a token *)
@@ -487,26 +492,26 @@ Module ParserFn (Import D : Defs.T).
           if t_eq_dec a' a then
             let p_stk' := (PF (T a :: pre) (Leaf a l :: v), p_frs) in
             let s_stk' := (SF suf', s_frs)                         in
-            StepK_opt p_stk' s_stk' ts' (allNts g) u
+            StepK_opt p_stk' s_stk' ts' (allNts g) u c
           else
             StepReject_opt "token mismatch"
         end
       (* nonterminal case --> push a frame onto the stack *)
       | NT x :: _ => 
         if NtSet.mem x av then
-          match adaptivePredict g cm x s_stk ts with
-          | PredSucc rhs =>
+          match adaptivePredict g cm x s_stk ts c with
+          | (PredSucc rhs, c') =>
             let p_stk' := (PF [] [], PF pre v :: p_frs) in
             let s_stk' := (SF rhs, SF suf :: s_frs)     in
-            StepK_opt p_stk' s_stk' ts (NtSet.remove x av) u
-          | PredAmbig rhs =>
+            StepK_opt p_stk' s_stk' ts (NtSet.remove x av) u c'
+          | (PredAmbig rhs, _) =>
             let p_stk' := (PF [] [], PF pre v :: p_frs) in
             let s_stk' := (SF rhs, SF suf :: s_frs)     in
-            StepK_opt p_stk' s_stk' ts (NtSet.remove x av) false
-          | PredReject =>
+            StepK_opt p_stk' s_stk' ts (NtSet.remove x av) false c
+          | (PredReject, _) =>
             StepReject_opt "prediction found no viable right-hand sides"
-          | PredError e =>
-            StepError_opt (PredictionError e)
+          | (PredError e, _) =>
+            StepError_opt (PredictionError e) 
           end
         else if NtSet.mem x (allNts g) then
                StepError_opt (LeftRecursion x)
@@ -541,8 +546,8 @@ Module ParserFn (Import D : Defs.T).
   Axiom magic : forall A, A.
     
   Lemma StepK_result_acc_opt :
-    forall g cm ps ps' ss ss' ts ts' av av' u u' (a : Acc lex_nat_triple (meas g ss ts av)),
-      step_opt g cm ps ss ts av u = StepK_opt ps' ss' ts' av' u'
+    forall g cm ps ps' ss ss' ts ts' av av' u u' c c' (a : Acc lex_nat_triple (meas g ss ts av)),
+      step_opt g cm ps ss ts av u c = StepK_opt ps' ss' ts' av' u' c'
       -> Acc lex_nat_triple (meas g ss' ts' av').
   Proof.
     intros; eapply Acc_inv; eauto.
@@ -556,21 +561,22 @@ Module ParserFn (Import D : Defs.T).
                          (ts : list token)
                          (av : NtSet.t)
                          (u  : bool)
+                         (c  : cache)
                          (a  : Acc lex_nat_triple (meas g ss ts av))
                          {struct a} : parse_result :=
-    match step_opt g cm ps ss ts av u as res return step_opt g cm ps ss ts av u = res -> _ with
+    match step_opt g cm ps ss ts av u c as res return step_opt g cm ps ss ts av u c = res -> _ with
     | StepAccept_opt v             => fun _  => if u then Accept v else Ambig v
     | StepReject_opt s             => fun _  => Reject s
     | StepError_opt e              => fun _  => Error e
-    | StepK_opt ps' ss' ts' av' u' =>
-      fun hs => multistep_opt g cm ps' ss' ts' av' u'
-                              (StepK_result_acc_opt _ _ _ _ _ _ _ _ _ _ _ _ a hs)
+    | StepK_opt ps' ss' ts' av' u' c' =>
+      fun hs => multistep_opt g cm ps' ss' ts' av' u' c'
+                              (StepK_result_acc_opt _ _ _ _ _ _ _ _ _ _ _ _ _ _ a hs)
     end eq_refl.
   
   Definition parse_opt (g : grammar) (gamma : list symbol) (ts : list token) : parse_result :=
-    let cm     := PC.PEF.P.SLL.mkGraph g      in
+    let cm     := PC.PEF.P.SLL.mkGraph g in
     let p_stk0 := (PF [] [], []) in
     let s_stk0 := (SF gamma, []) in
-    multistep_opt g cm p_stk0 s_stk0 ts (allNts g) true (lex_nat_triple_wf _). 
+    multistep_opt g cm p_stk0 s_stk0 ts (allNts g) true empty_cache (lex_nat_triple_wf _). 
   
 End ParserFn.
